prove additional precondition within correctness.fst w/ induction_props required for evict*_simulates proofs

intermediate/Veritas.Intermediate.Correctness.fst
@@ -39,83 +39,83 @@ module SpecV = Veritas.Verifier
 module SpecTS = Veritas.Verifier.TSLog
 module SpecC = Veritas.Verifier.Correctness
 
-(* 
+(*
  * A bunch of properties we use in the induction step:
  *    (a) the intermediate verifiers all satisfy the store invariant
  *    (b) the intermediate and spec level verifiers states correspond to one-another (related)
  *    (c) the spec level log is time sorted (b and c imply that the spec log has type its_log)
- *    (d) the spec level log is evict-add-consistent 
+ *    (d) the spec level log is evict-add-consistent
  * TODO: rename this
  *)
-let induction_props #vcfg (ils: its_log vcfg) = 
+let induction_props #vcfg (ils: its_log vcfg) =
   let ilk = to_logk ils in
   spec_rel ils /\
   SpecTS.is_eac ilk
 
 
-let induction_props_or_hash_collision #vcfg (ils: its_log vcfg) = 
+let induction_props_or_hash_collision #vcfg (ils: its_log vcfg) =
   o:option hash_collision_gen{Some? o \/ induction_props ils}
 
-let inductive_step_get #vcfg 
-                       (ils: IntTS.hash_verifiable_log vcfg) 
+let inductive_step_get #vcfg
+                       (ils: IntTS.hash_verifiable_log vcfg)
                        (i:I.seq_index ils{let ils_i = I.prefix ils i in
                                               induction_props ils_i /\
-                                              IntL.Get_S? (I.index ils i)}): induction_props_or_hash_collision (I.prefix ils (i + 1)) = 
-  let ilk = to_logk ils in  
+                                              IntL.Get_S? (I.index ils i)}): induction_props_or_hash_collision (I.prefix ils (i + 1)) =
+  let ilk = to_logk ils in
   let ils_i = I.prefix ils i in
   let ilk_i = I.prefix ilk i in
   let ils_i1 = I.prefix ils (i + 1) in
-  let ilk_i1 = I.prefix ilk (i + 1) in  
+  let ilk_i1 = I.prefix ilk (i + 1) in
 
   let vss_i = thread_state_pre ils i in
-  let vsk_i = SpecTS.thread_state_pre ilk i in 
+  let vsk_i = SpecTS.thread_state_pre ilk i in
   let es = I.index ils i in
   SpecTS.lemma_verifier_thread_state_extend ilk i;
-  
+
   match es with
-  
+
   | Get_S s k v ->
     lemma_vget_simulates_spec vss_i vsk_i es;
-    lemma_forall_vtls_rel_extend ils i;    
+    lemma_forall_vtls_rel_extend ils i;
     lemma_vget_preserves_ismap vss_i es;
     lemma_forall_store_ismap_extend ils i;
-    
+
     if SpecTS.is_eac ilk_i1 then
-      None    
+      None
     else (
       SpecTS.lemma_eac_boundary_inv ilk_i1 i;
       Some (lemma_non_eac_get_implies_hash_collision ilk_i1)
     )
 
-let inductive_step_put #vcfg 
-                       (ils: IntTS.hash_verifiable_log vcfg) 
+let inductive_step_put #vcfg
+                       (ils: IntTS.hash_verifiable_log vcfg)
                        (i:I.seq_index ils{let ils_i = I.prefix ils i in
                                               induction_props ils_i /\
-                                              IntL.Put_S? (I.index ils i)}): induction_props_or_hash_collision (I.prefix ils (i + 1)) = 
-  let ilk = to_logk ils in  
+                                              IntL.Put_S? (I.index ils i)}): induction_props_or_hash_collision (I.prefix ils (i + 1)) =
+  let ilk = to_logk ils in
   let ils_i = I.prefix ils i in
   let ilk_i = I.prefix ilk i in
   let ils_i1 = I.prefix ils (i + 1) in
-  let ilk_i1 = I.prefix ilk (i + 1) in  
+  let ilk_i1 = I.prefix ilk (i + 1) in
 
   let vss_i = thread_state_pre ils i in
-  let vsk_i = SpecTS.thread_state_pre ilk i in 
+  let vsk_i = SpecTS.thread_state_pre ilk i in
   let es = I.index ils i in
   SpecTS.lemma_verifier_thread_state_extend ilk i;
-  
+
   match es with
-  
-  | Put_S s k v -> 
+
+  | Put_S s k v ->
     lemma_vput_simulates_spec vss_i vsk_i es;
-    lemma_forall_vtls_rel_extend ils i;        
+    lemma_forall_vtls_rel_extend ils i;
     lemma_vput_preserves_ismap vss_i es;
     lemma_forall_store_ismap_extend ils i;
     if SpecTS.is_eac ilk_i1 then
-      None    
+      None
     else (
       SpecTS.lemma_eac_boundary_inv ilk_i1 i;
       Some (lemma_non_eac_put_implies_hash_collision ilk_i1)
-    )  
+    )
 
 let lemma_induction_props_implies_vtls_rel #vcfg
                                            (ils: its_log vcfg)
@@ -125,30 +125,30 @@ let lemma_induction_props_implies_vtls_rel #vcfg
                     let vsk_i = SpecTS.thread_state_pre ilk i in
                     vtls_rel vss_i vsk_i))
           [SMTPat (I.prefix ils i)]
-  = ()                    
+  = ()
 
-let inductive_step_addm_caseA #vcfg 
-                              (ils: IntTS.hash_verifiable_log vcfg) 
+let inductive_step_addm_caseA #vcfg
+                              (ils: IntTS.hash_verifiable_log vcfg)
                               (i:I.seq_index ils{let ils_i = I.prefix ils i in
                                                  let vss_i = IntTS.thread_state_pre ils i in
                                                  let sts = IntV.thread_store vss_i in
                                                  induction_props ils_i /\
-                                                 AddM_S? (I.index ils i) /\                                                 
+                                                 AddM_S? (I.index ils i) /\
                                                  (let AddM_S s (k,v) s' = I.index ils i in
                                                   not (store_contains_key sts k))})
-  : induction_props_or_hash_collision (I.prefix ils (i + 1)) = 
-  let tid = IntTS.thread_id_of ils i in                                          
-  let ilk = to_logk ils in  
+  : induction_props_or_hash_collision (I.prefix ils (i + 1)) =
+  let tid = IntTS.thread_id_of ils i in
+  let ilk = to_logk ils in
   let ils_i = I.prefix ils i in
   let ilk_i = I.prefix ilk i in
   let ils_i1 = I.prefix ils (i + 1) in
-  let ilk_i1 = I.prefix ilk (i + 1) in  
+  let ilk_i1 = I.prefix ilk (i + 1) in
   let vss_i = thread_state_pre ils i in
   let vsk_i = SpecTS.thread_state_pre ilk i in
   let vsk_i1 = SpecTS.thread_state_post ilk i in
   let es = I.index ils i in
   SpecTS.lemma_verifier_thread_state_extend ilk i;
-  
+
   let ek = I.index ilk i in
 
   match es with
@@ -156,22 +156,22 @@ let inductive_step_addm_caseA #vcfg
     let sts = IntV.thread_store vss_i in
     let stk = SpecV.thread_store vsk_i in
     lemma_vaddm_preserves_spec_new_key vss_i vsk_i es;
-    lemma_forall_vtls_rel_extend ils i;              
+    lemma_forall_vtls_rel_extend ils i;
     lemma_vaddm_preserves_ismap_new_key vss_i es;
-    lemma_forall_store_ismap_extend ils i;      
+    lemma_forall_store_ismap_extend ils i;
     if SpecTS.is_eac ilk_i1 then
-      None    
+      None
     else (
       SpecTS.lemma_eac_boundary_inv ilk_i1 i;
       Some (lemma_non_eac_addm_implies_hash_collision ilk_i1)
-    )    
+    )
 
 
 //#push-options "--z3rlimit_factor 3"
 #push-options "--max_fuel 1 --max_ifuel 0"
 
-let inductive_step_addm_caseB #vcfg 
-                              (ils: IntTS.hash_verifiable_log vcfg)                               
+let inductive_step_addm_caseB #vcfg
+                              (ils: IntTS.hash_verifiable_log vcfg)
                               (i:I.seq_index ils)
                               (sk: slot_id vcfg)
                               (sk_anc: slot_id vcfg{let ils_i = I.prefix ils i in
@@ -182,15 +182,15 @@ let inductive_step_addm_caseB #vcfg
                                                     inuse_slot sts sk /\ inuse_slot sts sk_anc /\
                                                     (let AddM_S s (k,v) s' = I.index ils i in
                                                      let k_anc = stored_key sts sk_anc in
-                                                     let k' = stored_key sts s' in                                                      
+                                                     let k' = stored_key sts s' in
                                                      stored_key sts sk = k /\ k_anc = k' /\ points_to sts sk_anc sk)})
-  : induction_props_or_hash_collision (I.prefix ils (i + 1)) = 
+  : induction_props_or_hash_collision (I.prefix ils (i + 1)) =
   let tid = IntTS.thread_id_of ils i in
-  let ilk = to_logk ils in  
+  let ilk = to_logk ils in
   let ils_i = I.prefix ils i in
   let ilk_i = I.prefix ilk i in
   let ils_i1 = I.prefix ils (i + 1) in
-  let ilk_i1 = I.prefix ilk (i + 1) in  
+  let ilk_i1 = I.prefix ilk (i + 1) in
   let vss_i = thread_state_pre ils i in
   let vsk_i = SpecTS.thread_state_pre ilk i in
   let vsk_i1 = SpecTS.thread_state_post ilk i in
@@ -208,19 +208,19 @@ let inductive_step_addm_caseB #vcfg
     assert(slot_points_to_is_merkle_points_to sts);
     assert(slot_points_to_is_merkle_points_to_local sts sk_anc sk d_anc);
     assert(points_to_dir sts sk_anc d_anc sk);
-    
+
     let mv_anc = to_merkle_value (stored_value sts sk_anc) in
     // assert(mv_points_to mv_anc d_anc k);
 
     let k_anc = stored_key sts sk_anc in
     // assert(SpecV.store_contains stk k_anc);
-    // assert(SpecV.stored_value stk k_anc = stored_value sts sk_anc);    
-    SpecTS.lemma_eac_value_is_stored_value ilk_i k_anc tid;    
+    // assert(SpecV.stored_value stk k_anc = stored_value sts sk_anc);
+    SpecTS.lemma_eac_value_is_stored_value ilk_i k_anc tid;
     lemma_mv_points_to_dir_correct ilk_i k_anc d_anc;
     lemma_ismap_correct sts sk s';
     // assert(s' = sk_anc);
     None
-    
+
 #pop-options
 
 let proving_ancestor #vcfg
@@ -229,7 +229,7 @@ let proving_ancestor #vcfg
                      (s:slot_id vcfg{let ils_i = I.prefix ils i in
                                      let vss_i = thread_state_pre ils i in
                                      let sts = IntV.thread_store vss_i in
-                                     induction_props ils_i /\ 
+                                     induction_props ils_i /\
                                      inuse_slot sts s /\ stored_key sts s <> Root}):
   pk:merkle_key{let ils_i = I.prefix ils i in
                  let vss_i = thread_state_pre ils i in
@@ -237,13 +237,13 @@ let proving_ancestor #vcfg
                  let k = stored_key sts s in
                  let ilk = to_logk ils in
                  let ilk_i = I.prefix ilk i in
-                 pk = SpecM.proving_ancestor ilk_i k} = 
+                 pk = SpecM.proving_ancestor ilk_i k} =
   let tid = IntTS.thread_id_of ils i in
-  let ilk = to_logk ils in  
+  let ilk = to_logk ils in
   let ils_i = I.prefix ils i in
   let ilk_i = I.prefix ilk i in
   let vss_i = thread_state_pre ils i in
-  
+
   let sts = IntV.thread_store vss_i in
 
   let k = stored_key sts s in
@@ -251,8 +251,8 @@ let proving_ancestor #vcfg
 
 #push-options "--max_fuel 1 --max_ifuel 0"
 
-let inductive_step_addm_caseD #vcfg 
-                              (ils: IntTS.hash_verifiable_log vcfg)                               
+let inductive_step_addm_caseD #vcfg
+                              (ils: IntTS.hash_verifiable_log vcfg)
                               (i:I.seq_index ils)
                               (sk: slot_id vcfg{let ils_i = I.prefix ils i in
                                                 let vss_i = IntTS.thread_state_pre ils i in
@@ -262,16 +262,16 @@ let inductive_step_addm_caseD #vcfg
                                                 inuse_slot sts sk /\
                                                 add_method_of sts sk = BAdd /\
                                                 (let AddM_S s (k,v) s' = I.index ils i in
-                                                 let k' = stored_key sts s' in                                                 
+                                                 let k' = stored_key sts s' in
                                                  stored_key sts sk = k /\
                                                  k' = proving_ancestor ils i sk)})
-  : induction_props_or_hash_collision (I.prefix ils (i + 1)) = 
+  : induction_props_or_hash_collision (I.prefix ils (i + 1)) =
   let tid = IntTS.thread_id_of ils i in
-  let ilk = to_logk ils in  
+  let ilk = to_logk ils in
   let ils_i = I.prefix ils i in
   let ilk_i = I.prefix ilk i in
   let ils_i1 = I.prefix ils (i + 1) in
-  let ilk_i1 = I.prefix ilk (i + 1) in  
+  let ilk_i1 = I.prefix ilk (i + 1) in
   let vss_i = thread_state_pre ils i in
   let vsk_i = SpecTS.thread_state_pre ilk i in
   let vsk_i1 = SpecTS.thread_state_post ilk i in
@@ -281,9 +281,9 @@ let inductive_step_addm_caseD #vcfg
   let ek = I.index ilk i in
 
   match es with
-  | AddM_S s (k,v) s' -> 
+  | AddM_S s (k,v) s' ->
     let sts = IntV.thread_store vss_i in
-    let stk = SpecV.thread_store vsk_i in     
+    let stk = SpecV.thread_store vsk_i in
 
     lemma_addm_props vss_i es;
     let k' = stored_key sts s' in
@@ -298,7 +298,7 @@ let inductive_step_addm_caseD #vcfg
     assert (E.add_method_of (SpecTS.eac_state_of_key ilk_i k) = SpecTS.stored_add_method ilk_i k);
 
     let aux():
-      Lemma (SpecTS.stored_tid ilk_i k = tid) = 
+      Lemma (SpecTS.stored_tid ilk_i k = tid) =
       let tid' = SpecTS.stored_tid ilk_i k in
       if tid' = tid then ()
       else
@@ -309,16 +309,16 @@ let inductive_step_addm_caseD #vcfg
 
     SpecM.lemma_proving_ancestor_blum_bit ilk_i k;
     assert(SpecV.store_contains stk k');
-    SpecTS.lemma_eac_value_is_stored_value ilk_i k' tid;    
-    assert(mv_evicted_to_blum v' d);    
-    
+    SpecTS.lemma_eac_value_is_stored_value ilk_i k' tid;
+    assert(mv_evicted_to_blum v' d);
+
     assert(induction_props ils_i1);
-    None        
+    None
 
 #pop-options
 
-let inductive_step_addm_caseE #vcfg 
-                              (ils: IntTS.hash_verifiable_log vcfg)                               
+let inductive_step_addm_caseE #vcfg
+                              (ils: IntTS.hash_verifiable_log vcfg)
                               (i:I.seq_index ils)
                               (sk: slot_id vcfg{let ils_i = I.prefix ils i in
                                                 let vss_i = IntTS.thread_state_pre ils i in
@@ -327,16 +327,16 @@ let inductive_step_addm_caseE #vcfg
                                                 AddM_S? (I.index ils i) /\
                                                 inuse_slot sts sk /\
                                                 (let AddM_S s (k,v) s' = I.index ils i in
-                                                 let k' = stored_key sts s' in                                                 
+                                                 let k' = stored_key sts s' in
                                                  stored_key sts sk = k /\
                                                  k' <> proving_ancestor ils i sk)})
-  : induction_props_or_hash_collision (I.prefix ils (i + 1)) = 
+  : induction_props_or_hash_collision (I.prefix ils (i + 1)) =
   let tid = IntTS.thread_id_of ils i in
-  let ilk = to_logk ils in  
+  let ilk = to_logk ils in
   let ils_i = I.prefix ils i in
   let ilk_i = I.prefix ilk i in
   let ils_i1 = I.prefix ils (i + 1) in
-  let ilk_i1 = I.prefix ilk (i + 1) in  
+  let ilk_i1 = I.prefix ilk (i + 1) in
   let vss_i = thread_state_pre ils i in
   let vsk_i = SpecTS.thread_state_pre ilk i in
   let vsk_i1 = SpecTS.thread_state_post ilk i in
@@ -348,7 +348,7 @@ let inductive_step_addm_caseE #vcfg
   match es with
   | AddM_S s (k,v) s' ->
     let sts = IntV.thread_store vss_i in
-    let stk = SpecV.thread_store vsk_i in     
+    let stk = SpecV.thread_store vsk_i in
 
     lemma_addm_props vss_i es;
     let k' = stored_key sts s' in
@@ -356,8 +356,8 @@ let inductive_step_addm_caseE #vcfg
     let d = desc_dir k k' in
 
     let pk = proving_ancestor ils i sk in
-    let aux () 
-      : Lemma (k' = Root \/ not (SpecTS.is_eac_state_init ilk_i k')) = 
+    let aux ()
+      : Lemma (k' = Root \/ not (SpecTS.is_eac_state_init ilk_i k')) =
       if k' = Root then ()
       else (
         assert(SpecV.store_contains stk k');
@@ -374,26 +374,26 @@ let inductive_step_addm_caseE #vcfg
     assert(is_desc k2 k);
     lemma_desc_depth_monotonic k2 k;
     assert(is_desc pk k2);
-    lemma_desc_depth_monotonic pk k2;    
-    None    
+    lemma_desc_depth_monotonic pk k2;
+    None
 
-let inductive_step_addm #vcfg 
-                       (ils: IntTS.hash_verifiable_log vcfg) 
+let inductive_step_addm #vcfg
+                       (ils: IntTS.hash_verifiable_log vcfg)
                        (i:I.seq_index ils{let ils_i = I.prefix ils i in
                                           induction_props ils_i /\
-                                          AddM_S? (I.index ils i)}): induction_props_or_hash_collision (I.prefix ils (i + 1)) = 
-  let tid = IntTS.thread_id_of ils i in                                          
-  let ilk = to_logk ils in  
+                                          AddM_S? (I.index ils i)}): induction_props_or_hash_collision (I.prefix ils (i + 1)) =
+  let tid = IntTS.thread_id_of ils i in
+  let ilk = to_logk ils in
   let ils_i = I.prefix ils i in
   let ilk_i = I.prefix ilk i in
   let ils_i1 = I.prefix ils (i + 1) in
-  let ilk_i1 = I.prefix ilk (i + 1) in  
+  let ilk_i1 = I.prefix ilk (i + 1) in
   let vss_i = thread_state_pre ils i in
   let vsk_i = SpecTS.thread_state_pre ilk i in
   let vsk_i1 = SpecTS.thread_state_post ilk i in
   let es = I.index ils i in
   SpecTS.lemma_verifier_thread_state_extend ilk i;
-  
+
   let ek = I.index ilk i in
 
   match es with
@@ -401,7 +401,7 @@ let inductive_step_addm #vcfg
     let sts = IntV.thread_store vss_i in
     let stk = SpecV.thread_store vsk_i in
     let k' = stored_key sts s' in
-    
+
     if store_contains_key sts k then
       let sk = slot_of_key sts k in
       let pk = proving_ancestor ils i sk in
@@ -413,57 +413,57 @@ let inductive_step_addm #vcfg
 
         let d_anc = if points_to_dir sts sk_anc Left sk then Left else Right in
         assert(slot_points_to_is_merkle_points_to_local sts sk_anc sk d_anc);
-        // let mv_anc = to_merkle_value (stored_value sts sk_anc) in        
+        // let mv_anc = to_merkle_value (stored_value sts sk_anc) in
         let k_anc = stored_key sts sk_anc in
 
         SpecTS.lemma_eac_value_is_stored_value ilk_i k_anc tid;
         // assert(mv_anc = eac_merkle_value ilk_i k_anc);
         lemma_points_to_implies_proving_ancestor ilk_i k k_anc d_anc;
         // assert(k_anc = SpecM.proving_ancestor ilk_i k);
-        
+
         inductive_step_addm_caseB ils i sk sk_anc
       )
-      else 
+      else
         inductive_step_addm_caseD ils i sk
-    
-    else 
+
+    else
       inductive_step_addm_caseA ils i
 
-let inductive_step_evictm #vcfg 
-                       (ils: IntTS.hash_verifiable_log vcfg) 
+let inductive_step_evictm #vcfg
+                       (ils: IntTS.hash_verifiable_log vcfg)
                        (i:I.seq_index ils{let ils_i = I.prefix ils i in
                                           induction_props ils_i /\
-                                          EvictM_S? (I.index ils i)}): induction_props_or_hash_collision (I.prefix ils (i + 1)) = 
-  let tid = IntTS.thread_id_of ils i in                                          
-  let ilk = to_logk ils in  
+                                          EvictM_S? (I.index ils i)}): induction_props_or_hash_collision (I.prefix ils (i + 1)) =
+  let tid = IntTS.thread_id_of ils i in
+  let ilk = to_logk ils in
   let ils_i = I.prefix ils i in
   let ilk_i = I.prefix ilk i in
   let ils_i1 = I.prefix ils (i + 1) in
-  let ilk_i1 = I.prefix ilk (i + 1) in  
+  let ilk_i1 = I.prefix ilk (i + 1) in
   let vss_i = thread_state_pre ils i in
   let vsk_i = SpecTS.thread_state_pre ilk i in
   let vsk_i1 = SpecTS.thread_state_post ilk i in
   let es = I.index ils i in
   SpecTS.lemma_verifier_thread_state_extend ilk i;
-  
+
   let ek = I.index ilk i in
 
   match es with
   | EvictM_S s s' ->
     lemma_evictm_simulates_spec vss_i vsk_i es;
-    lemma_forall_vtls_rel_extend ils i;    
+    lemma_forall_vtls_rel_extend ils i;
     lemma_evictm_preserves_ismap vss_i es;
     lemma_forall_store_ismap_extend ils i;
-    
+
     if SpecTS.is_eac ilk_i1 then
-      None    
+      None
     else (
       SpecTS.lemma_eac_boundary_inv ilk_i1 i;
       Some (lemma_non_eac_evictm_implies_hash_collision ilk_i1)
     )
 
-let inductive_step_addb_neac_caseA #vcfg 
-                       (ils: IntTS.hash_verifiable_log vcfg) 
+let inductive_step_addb_neac_caseA #vcfg
+                       (ils: IntTS.hash_verifiable_log vcfg)
                        (i:I.seq_index ils{let ils_i = I.prefix ils i in
                                           let ils_i1 = I.prefix ils (i + 1) in
                                           let vss_i = IntTS.thread_state_pre ils i in
@@ -476,21 +476,21 @@ let inductive_step_addb_neac_caseA #vcfg
                                           not (SpecTS.is_eac ilk_i1) /\
                                           SpecTS.is_eac ilk_i /\
                                           E.EACInit? (SpecTS.eac_state_pre ilk_i1 i)
-                                          }): hash_collision_gen = 
-  let gl = g_logS_of ils in                                          
+                                          }): hash_collision_gen =
+  let gl = g_logS_of ils in
   let ils_i = I.prefix ils i in
   let ils_i1 = I.prefix ils (i + 1) in
   let vss_i = IntTS.thread_state_pre ils i in
-  let sts = IntV.thread_store vss_i in        
+  let sts = IntV.thread_store vss_i in
   let ilk_i = to_logk ils_i in
-  let ilk_i1 = to_logk ils_i1 in  
+  let ilk_i1 = to_logk ils_i1 in
   SpecTS.lemma_eac_boundary_inv ilk_i1 i;
   assert(SpecTS.eac_boundary ilk_i1 = i);
   let st = SpecTS.eac_state_pre ilk_i1 i in
   let ee = SpecTS.vlog_entry_ext_at ilk_i1 i in
   let es = I.index ils i in
   let ek = I.index ilk_i1 i in
-  
+
   match es with
   | AddB_S s (k, v) t j ->
     // assert(ek = AddB (k, v) t j);
@@ -505,11 +505,11 @@ let inductive_step_addb_neac_caseA #vcfg
       IntB.lemma_evict_before_add ils i;
       // assert(j < i);
       // the following assert needed to trigger smtpat
-      assert(I.index ils j = I.index ils_i j);      
-      
+      assert(I.index ils j = I.index ils_i j);
+
       // assert(IntTS.to_logK_entry ils j = I.index ilk_i1 j);
       // assert(be = IntB.blum_evict_elem ils j);
-      lemma_blum_evict_elem ils i j;    
+      lemma_blum_evict_elem ils i j;
       // assert(be = IntB.blum_evict_elem ils_i j);
       lemma_spec_rel_implies_same_evict_elem ils_i j;
       // assert(be = SpecB.blum_evict_elem ilk_i j);
@@ -519,7 +519,7 @@ let inductive_step_addb_neac_caseA #vcfg
       lemma_last_index_correct2 (SpecTS.is_entry_of_key k) (I.i_seq ilk_i) j;
       hash_collision_contra()
     )
-    else (      
+    else (
       // assert(IntB.add_set ils `contains` be);
       // assert(IntB.add_set ils == IntG.add_set gl);
       // assert(IntB.evict_set ils == IntG.evict_set gl);
@@ -527,8 +527,8 @@ let inductive_step_addb_neac_caseA #vcfg
       MultiHashCollision (MSCollision (IntG.add_seq gl) (IntG.evict_seq gl))
     )
 
-let inductive_step_addb_neac_caseB #vcfg 
-                       (ils: IntTS.hash_verifiable_log vcfg) 
+let inductive_step_addb_neac_caseB #vcfg
+                       (ils: IntTS.hash_verifiable_log vcfg)
                        (i:I.seq_index ils{let ils_i = I.prefix ils i in
                                           let ils_i1 = I.prefix ils (i + 1) in
                                           let vss_i = IntTS.thread_state_pre ils i in
@@ -541,10 +541,10 @@ let inductive_step_addb_neac_caseB #vcfg
                                           not (SpecTS.is_eac ilk_i1) /\
                                           SpecTS.is_eac ilk_i /\
                                           E.EACInStore? (SpecTS.eac_state_pre ilk_i1 i)
-                                          }): hash_collision_gen = 
-  let gl = g_logS_of ils in                                          
+                                          }): hash_collision_gen =
+  let gl = g_logS_of ils in
   let ils_i1 = I.prefix ils (i + 1) in
-  let ilk_i1 = to_logk ils_i1 in  
+  let ilk_i1 = to_logk ils_i1 in
   SpecTS.lemma_eac_boundary_inv ilk_i1 i;
   let es = I.index ils i in
 
@@ -552,12 +552,12 @@ let inductive_step_addb_neac_caseB #vcfg
   | AddB_S s (k, v) t j ->
     let be = SpecB.eac_instore_addb_diff_elem ilk_i1 i in
     // triggers some SMTPat ...
-    let _ = I.prefix ilk_i1 (i + 1) in        
+    let _ = I.prefix ilk_i1 (i + 1) in
     lemma_add_delta_implies_not_eq ils (i + 1) be;
     MultiHashCollision (MSCollision (IntG.add_seq gl) (IntG.evict_seq gl))
 
-let inductive_step_addb_neac_caseC #vcfg 
-                       (ils: IntTS.hash_verifiable_log vcfg) 
+let inductive_step_addb_neac_caseC #vcfg
+                       (ils: IntTS.hash_verifiable_log vcfg)
                        (i:I.seq_index ils{let ils_i = I.prefix ils i in
                                           let ils_i1 = I.prefix ils (i + 1) in
                                           let vss_i = IntTS.thread_state_pre ils i in
@@ -570,10 +570,10 @@ let inductive_step_addb_neac_caseC #vcfg
                                           not (SpecTS.is_eac ilk_i1) /\
                                           SpecTS.is_eac ilk_i /\
                                           E.EACEvictedMerkle? (SpecTS.eac_state_pre ilk_i1 i)
-                                          }): hash_collision_gen = 
-  let gl = g_logS_of ils in                                          
+                                          }): hash_collision_gen =
+  let gl = g_logS_of ils in
   let ils_i1 = I.prefix ils (i + 1) in
-  let ilk_i1 = to_logk ils_i1 in  
+  let ilk_i1 = to_logk ils_i1 in
   SpecTS.lemma_eac_boundary_inv ilk_i1 i;
   let es = I.index ils i in
 
@@ -581,12 +581,12 @@ let inductive_step_addb_neac_caseC #vcfg
   | AddB_S s (k, v) t j ->
     let be = SpecB.eac_evictedm_addb_diff_elem ilk_i1 i in
     // triggers some SMTPat ...
-    let _ = I.prefix ilk_i1 (i + 1) in        
+    let _ = I.prefix ilk_i1 (i + 1) in
     lemma_add_delta_implies_not_eq ils (i + 1) be;
-    MultiHashCollision (MSCollision (IntG.add_seq gl) (IntG.evict_seq gl))                                          
-    
-let inductive_step_addb_neac_caseD #vcfg 
-                       (ils: IntTS.hash_verifiable_log vcfg) 
+    MultiHashCollision (MSCollision (IntG.add_seq gl) (IntG.evict_seq gl))
+
+let inductive_step_addb_neac_caseD #vcfg
+                       (ils: IntTS.hash_verifiable_log vcfg)
                        (i:I.seq_index ils{let ils_i = I.prefix ils i in
                                           let ils_i1 = I.prefix ils (i + 1) in
                                           let vss_i = IntTS.thread_state_pre ils i in
@@ -599,10 +599,10 @@ let inductive_step_addb_neac_caseD #vcfg
                                           not (SpecTS.is_eac ilk_i1) /\
                                           SpecTS.is_eac ilk_i /\
                                           E.EACEvictedBlum? (SpecTS.eac_state_pre ilk_i1 i)
-                                          }): hash_collision_gen = 
-  let gl = g_logS_of ils in                                          
+                                          }): hash_collision_gen =
+  let gl = g_logS_of ils in
   let ils_i1 = I.prefix ils (i + 1) in
-  let ilk_i1 = to_logk ils_i1 in  
+  let ilk_i1 = to_logk ils_i1 in
   SpecTS.lemma_eac_boundary_inv ilk_i1 i;
   let es = I.index ils i in
 
@@ -610,12 +610,12 @@ let inductive_step_addb_neac_caseD #vcfg
   | AddB_S s (k, v) t j ->
     let be = SpecB.eac_evictedb_addb_diff_elem ilk_i1 i in
     // triggers some SMTPat ...
-    let _ = I.prefix ilk_i1 (i + 1) in        
+    let _ = I.prefix ilk_i1 (i + 1) in
     lemma_add_delta_implies_not_eq ils (i + 1) be;
     MultiHashCollision (MSCollision (IntG.add_seq gl) (IntG.evict_seq gl))
 
-let inductive_step_addb_neac #vcfg 
-                       (ils: IntTS.hash_verifiable_log vcfg) 
+let inductive_step_addb_neac #vcfg
+                       (ils: IntTS.hash_verifiable_log vcfg)
                        (i:I.seq_index ils{let ils_i = I.prefix ils i in
                                           let ils_i1 = I.prefix ils (i + 1) in
                                           let vss_i = IntTS.thread_state_pre ils i in
@@ -630,15 +630,15 @@ let inductive_step_addb_neac #vcfg
   let ils_i = I.prefix ils i in
   let ils_i1 = I.prefix ils (i + 1) in
   let vss_i = IntTS.thread_state_pre ils i in
-  let sts = IntV.thread_store vss_i in                       
-  let ilk_i1 = to_logk ils_i1 in  
+  let sts = IntV.thread_store vss_i in
+  let ilk_i1 = to_logk ils_i1 in
   SpecTS.lemma_eac_boundary_inv ilk_i1 i;
   assert(SpecTS.eac_boundary ilk_i1 = i);
   let st = SpecTS.eac_state_pre ilk_i1 i in
   let ee = SpecTS.vlog_entry_ext_at ilk_i1 i in
   let es = I.index ils i in
   let ek = I.index ilk_i1 i in
-  
+
   match es with
   | AddB_S s (k, v) t j ->
     // assert(ek = AddB (k, v) t j);
@@ -662,34 +662,34 @@ let inductive_step_addb_neac #vcfg
       | E.NEvict (AddB _ _ _) -> inductive_step_addb_neac_caseD ils i
       )
 
-let inductive_step_addb_caseA #vcfg 
-                       (ils: IntTS.hash_verifiable_log vcfg) 
+let inductive_step_addb_caseA #vcfg
+                       (ils: IntTS.hash_verifiable_log vcfg)
                        (i:I.seq_index ils{let ils_i = I.prefix ils i in
                                           let vss_i = IntTS.thread_state_pre ils i in
-                                          let sts = IntV.thread_store vss_i in                       
+                                          let sts = IntV.thread_store vss_i in
                                           induction_props ils_i /\
                                           AddB_S? (I.index ils i) /\
                                           (let AddB_S _ (k,_) _ _ = I.index ils i in
-                                           not (store_contains_key sts k)                                          
-                                          )}): induction_props_or_hash_collision (I.prefix ils (i + 1)) = 
-  let tid = IntTS.thread_id_of ils i in                                          
-  let ilk = to_logk ils in  
+                                           not (store_contains_key sts k)
+                                          )}): induction_props_or_hash_collision (I.prefix ils (i + 1)) =
+  let tid = IntTS.thread_id_of ils i in
+  let ilk = to_logk ils in
   let ils_i = I.prefix ils i in
   let ilk_i = I.prefix ilk i in
   let ils_i1 = I.prefix ils (i + 1) in
-  let ilk_i1 = I.prefix ilk (i + 1) in  
+  let ilk_i1 = I.prefix ilk (i + 1) in
   let vss_i = thread_state_pre ils i in
   let vsk_i = SpecTS.thread_state_pre ilk i in
   let vsk_i1 = SpecTS.thread_state_post ilk i in
   let es = I.index ils i in
   SpecTS.lemma_verifier_thread_state_extend ilk i;
-  
+
   let ek = I.index ilk i in
 
   match es with
   | AddB_S s (k,v) t j ->
     lemma_vaddb_preserves_spec_new_key vss_i vsk_i es;
-    lemma_forall_vtls_rel_extend ils i;    
+    lemma_forall_vtls_rel_extend ils i;
     lemma_vaddb_preserves_ismap_new_key vss_i es;
     lemma_forall_store_ismap_extend ils i;
 
@@ -700,29 +700,29 @@ let inductive_step_addb_caseA #vcfg
 #push-options "--max_fuel 1 --max_ifuel 0 --z3rlimit_factor 2"
 
 // TODO: extremely unstable proof - debug
-let inductive_step_addb_caseB #vcfg 
-                       (ils: IntTS.hash_verifiable_log vcfg) 
+let inductive_step_addb_caseB #vcfg
+                       (ils: IntTS.hash_verifiable_log vcfg)
                        (i:I.seq_index ils{let ils_i = I.prefix ils i in
                                           let vss_i = IntTS.thread_state_pre ils i in
-                                          let sts = IntV.thread_store vss_i in                       
+                                          let sts = IntV.thread_store vss_i in
                                           induction_props ils_i /\
                                           AddB_S? (I.index ils i) /\
                                           (let AddB_S _ (k,_) _ _ = I.index ils i in
                                            store_contains_key sts k
-                                          )}): induction_props_or_hash_collision (I.prefix ils (i + 1)) = 
+                                          )}): induction_props_or_hash_collision (I.prefix ils (i + 1)) =
   let gl = g_logS_of ils in
-  let tid = IntTS.thread_id_of ils i in                                          
-  let ilk = to_logk ils in  
+  let tid = IntTS.thread_id_of ils i in
+  let ilk = to_logk ils in
   let ils_i = I.prefix ils i in
   let ilk_i = I.prefix ilk i in
   let ils_i1 = I.prefix ils (i + 1) in
-  let ilk_i1 = I.prefix ilk (i + 1) in  
+  let ilk_i1 = I.prefix ilk (i + 1) in
   let vss_i = thread_state_pre ils i in
   let vsk_i = SpecTS.thread_state_pre ilk i in
   let vsk_i1 = SpecTS.thread_state_post ilk i in
   let es = I.index ils i in
   SpecTS.lemma_verifier_thread_state_extend ilk i;
-  
+
   let ek = I.index ilk i in
   // assert(forall_vtls_rel ils_i);
   assert(ilk_i == to_logk ils_i);
@@ -744,122 +744,172 @@ let inductive_step_addb_caseB #vcfg
 
     // assert(IntB.add_set ils_i1 == MS.add_elem (IntB.add_set ils_i) be);
     lemma_add_incr_mem (IntB.add_set ils_i) be;
-    IntB.lemma_evict_set_extend2 ils_i1;    
+    IntB.lemma_evict_set_extend2 ils_i1;
     // assert(MS.mem be (IntB.add_set ils_i1) > MS.mem be (IntB.evict_set ils_i));
     lemma_add_delta_implies_not_eq ils (i + 1) be;
     Some (MultiHashCollision (MSCollision (IntG.add_seq gl) (IntG.evict_seq gl)))
-    
+
 #pop-options
 
-let inductive_step_addb #vcfg 
-                       (ils: IntTS.hash_verifiable_log vcfg) 
+let inductive_step_addb #vcfg
+                       (ils: IntTS.hash_verifiable_log vcfg)
                        (i:I.seq_index ils{let ils_i = I.prefix ils i in
                                           let vss_i = IntTS.thread_state_pre ils i in
-                                          let sts = IntV.thread_store vss_i in                       
+                                          let sts = IntV.thread_store vss_i in
                                           induction_props ils_i /\
-                                          AddB_S? (I.index ils i) 
-                                          }): induction_props_or_hash_collision (I.prefix ils (i + 1)) = 
-  let tid = IntTS.thread_id_of ils i in                                          
-  let ilk = to_logk ils in  
+                                          AddB_S? (I.index ils i)
+                                          }): induction_props_or_hash_collision (I.prefix ils (i + 1)) =
+  let tid = IntTS.thread_id_of ils i in
+  let ilk = to_logk ils in
   let ils_i = I.prefix ils i in
   let ilk_i = I.prefix ilk i in
   let ils_i1 = I.prefix ils (i + 1) in
-  let ilk_i1 = I.prefix ilk (i + 1) in  
+  let ilk_i1 = I.prefix ilk (i + 1) in
   let vss_i = thread_state_pre ils i in
   let vsk_i = SpecTS.thread_state_pre ilk i in
   let vsk_i1 = SpecTS.thread_state_post ilk i in
   let es = I.index ils i in
   SpecTS.lemma_verifier_thread_state_extend ilk i;
-  
+
   let ek = I.index ilk i in
 
   match es with
   | AddB_S s (k,v) t j ->
     let sts = IntV.thread_store vss_i in
-    if store_contains_key sts k then 
+    if store_contains_key sts k then
       inductive_step_addb_caseB ils i
     else
       inductive_step_addb_caseA ils i
 
+let induction_props_implies_proving_ancestor #vcfg
+  (ils: IntTS.hash_verifiable_log vcfg)
+  (i: I.seq_index ils{let ils_i = I.prefix ils i in
+                      induction_props ils_i}):
+  Lemma (ensures (let vss = thread_state_pre ils i in
+                  let sts = IntV.thread_store vss in
+                  merkle_points_to_uniq sts)) =
+  let tid = IntTS.thread_id_of ils i in
+  let vss = thread_state_pre ils i in
+  let sts = IntV.thread_store vss in
+  let ilk = to_logk ils in
+  let ilk_i = I.prefix ilk i in
+  let vsk = SpecTS.thread_state_pre ilk i in
+  let stk = SpecV.thread_store vsk in
+  assert(store_rel sts stk);
 
-let inductive_step_evictb #vcfg 
-                       (ils: IntTS.hash_verifiable_log vcfg) 
+  let aux (s1 s2: _) (k: _)
+    : Lemma (ensures (merkle_points_to_uniq_local sts s1 s2 k))
+            [SMTPat (merkle_points_to_uniq_local sts s1 s2 k)] =
+    if merkle_points_to_uniq_local sts s1 s2 k then ()
+    else (
+      let mv1 = to_merkle_value (stored_value sts s1) in
+      let k1 = stored_key sts s1 in
+      let d1 = if mv_points_to mv1 Left k then Left else Right in
+      let mv2 = to_merkle_value (stored_value sts s2) in
+      let d2 = if mv_points_to mv2 Left k then Left else Right in
+      let k2 = stored_key sts s2 in
+      assert(mv_points_to mv1 d1 k);
+      assert(mv_points_to mv2 d2 k);
+
+      (* sts is a map store, so all keys are distinct *)
+      assert(k1 <> k2);
+
+      (* stk contains both keys k1 and k2 *)
+      assert(SpecV.store_contains stk k1);
+      assert(SpecV.store_contains stk k2);
+
+      assert(SpecV.stored_value stk k1 = stored_value sts s1);
+      assert(SpecV.stored_value stk k2 = stored_value sts s2);
+
+      SpecTS.lemma_eac_value_is_stored_value ilk_i k1 tid;
+      SpecTS.lemma_eac_value_is_stored_value ilk_i k2 tid;
+
+      SpecM.lemma_points_to_implies_proving_ancestor ilk_i k k1 d1;
+      SpecM.lemma_points_to_implies_proving_ancestor ilk_i k k2 d2;
+
+      ()
+    )
+  in
+  ()
+
+let inductive_step_evictb #vcfg
+                       (ils: IntTS.hash_verifiable_log vcfg)
                        (i:I.seq_index ils{let ils_i = I.prefix ils i in
                                           induction_props ils_i /\
-                                          EvictB_S? (I.index ils i)}): induction_props_or_hash_collision (I.prefix ils (i + 1)) = 
-  let tid = IntTS.thread_id_of ils i in                                          
-  let ilk = to_logk ils in  
+                                          EvictB_S? (I.index ils i)}): induction_props_or_hash_collision (I.prefix ils (i + 1)) =
+  let tid = IntTS.thread_id_of ils i in
+  let ilk = to_logk ils in
   let ils_i = I.prefix ils i in
   let ilk_i = I.prefix ilk i in
   let ils_i1 = I.prefix ils (i + 1) in
-  let ilk_i1 = I.prefix ilk (i + 1) in  
+  let ilk_i1 = I.prefix ilk (i + 1) in
   let vss_i = thread_state_pre ils i in
   let vsk_i = SpecTS.thread_state_pre ilk i in
   let vsk_i1 = SpecTS.thread_state_post ilk i in
   let es = I.index ils i in
   SpecTS.lemma_verifier_thread_state_extend ilk i;
-  
+
   let ek = I.index ilk i in
 
   match es with
   | EvictB_S s t ->
     lemma_evictb_simulates_spec vss_i vsk_i es;
-    lemma_forall_vtls_rel_extend ils i;        
-    lemma_evictb_preserves_ismap vss_i es;    
-    lemma_forall_store_ismap_extend ils i;    
+    lemma_forall_vtls_rel_extend ils i;
+    lemma_evictb_preserves_ismap vss_i es;
+    lemma_forall_store_ismap_extend ils i;
     if SpecTS.is_eac ilk_i1 then
-      None    
+      None
     else (
       SpecTS.lemma_eac_boundary_inv ilk_i1 i;
       Some (lemma_non_eac_evictb_implies_hash_collision ilk_i1)
     )
 
 
-let inductive_step_evictbm #vcfg 
-                       (ils: IntTS.hash_verifiable_log vcfg) 
+let inductive_step_evictbm #vcfg
+                       (ils: IntTS.hash_verifiable_log vcfg)
                        (i:I.seq_index ils{let ils_i = I.prefix ils i in
                                           induction_props ils_i /\
-                                          EvictBM_S? (I.index ils i)}): induction_props_or_hash_collision (I.prefix ils (i + 1)) = 
-  let tid = IntTS.thread_id_of ils i in                                          
-  let ilk = to_logk ils in  
+                                          EvictBM_S? (I.index ils i)}): induction_props_or_hash_collision (I.prefix ils (i + 1)) =
+  let tid = IntTS.thread_id_of ils i in
+  let ilk = to_logk ils in
   let ils_i = I.prefix ils i in
   let ilk_i = I.prefix ilk i in
   let ils_i1 = I.prefix ils (i + 1) in
-  let ilk_i1 = I.prefix ilk (i + 1) in  
+  let ilk_i1 = I.prefix ilk (i + 1) in
   let vss_i = thread_state_pre ils i in
   let vsk_i = SpecTS.thread_state_pre ilk i in
   let vsk_i1 = SpecTS.thread_state_post ilk i in
   let es = I.index ils i in
   SpecTS.lemma_verifier_thread_state_extend ilk i;
-  
+
   let ek = I.index ilk i in
 
   match es with
   | EvictBM_S s s' t ->
     lemma_evictbm_simulates_spec vss_i vsk_i es;
-    lemma_forall_vtls_rel_extend ils i;        
-    lemma_evictbm_preserves_ismap vss_i es;    
-    lemma_forall_store_ismap_extend ils i;    
+    lemma_forall_vtls_rel_extend ils i;
+    lemma_evictbm_preserves_ismap vss_i es;
+    lemma_forall_store_ismap_extend ils i;
     if SpecTS.is_eac ilk_i1 then
-      None    
+      None
     else (
       SpecTS.lemma_eac_boundary_inv ilk_i1 i;
       Some (lemma_non_eac_evictbm_implies_hash_collision ilk_i1)
     )
 
-(* 
- * induction step: if all the induction properties hold for prefix of length i, 
- * then the properties hold for prefix of length (i + 1) or we construct 
+(*
+ * induction step: if all the induction properties hold for prefix of length i,
+ * then the properties hold for prefix of length (i + 1) or we construct
  * a hash collision
  *)
-let inductive_step #vcfg 
-                   (ils: IntTS.hash_verifiable_log vcfg) 
+let inductive_step #vcfg
+                   (ils: IntTS.hash_verifiable_log vcfg)
                    (i:I.seq_index ils{let ils_i = I.prefix ils i in
-                                      induction_props ils_i}): induction_props_or_hash_collision (I.prefix ils (i + 1)) = 
-  let es = I.index ils i in 
+                                      induction_props ils_i}): induction_props_or_hash_collision (I.prefix ils (i + 1)) =
+  let es = I.index ils i in
   match es with
   | Get_S _ _ _ -> inductive_step_get ils i
-  | Put_S _ _ _ -> inductive_step_put ils i  
+  | Put_S _ _ _ -> inductive_step_put ils i
   | AddM_S _ _ _ -> inductive_step_addm ils i
   | EvictM_S _ _ -> inductive_step_evictm ils i
   | AddB_S _ _ _ _ -> inductive_step_addb ils i
@@ -867,60 +917,60 @@ let inductive_step #vcfg
   | EvictBM_S _ _ _  -> inductive_step_evictbm ils i
 
 let lemma_empty_implies_induction_props #vcfg (ils: its_log vcfg{I.length ils = 0})
-  : Lemma (ensures (induction_props ils)) 
-  = 
+  : Lemma (ensures (induction_props ils))
+  =
   IntTS.lemma_empty_implies_spec_rel ils;
   SpecTS.lemma_empty_log_eac (to_logk ils);
-  ()          
+  ()
 
-let rec lemma_hash_verifiable_implies_induction_props_or_hash_collision_aux 
-        #vcfg 
+let rec lemma_hash_verifiable_implies_induction_props_or_hash_collision_aux
+        #vcfg
         (ils: hash_verifiable_log vcfg)
         (i:nat{i <= I.length ils})
   : Tot (induction_props_or_hash_collision (I.prefix ils i))
-    (decreases i) = 
+    (decreases i) =
   let ils_i = I.prefix ils i in
   if i = 0 then (
      lemma_empty_implies_induction_props ils_i;
      None
   )
-  else 
+  else
     let hc_or_props = lemma_hash_verifiable_implies_induction_props_or_hash_collision_aux ils (i - 1) in
-    
+
     (* we found a hash collision - simply return the same *)
     if Some? hc_or_props then
       Some (Some?.v hc_or_props)
     else
       inductive_step ils (i - 1)
-  
+
 let lemma_hash_verifiable_implies_induction_props_or_hash_collision #vcfg (ils: hash_verifiable_log vcfg)
-  : induction_props_or_hash_collision ils = 
+  : induction_props_or_hash_collision ils =
   I.lemma_fullprefix_equal ils;
   lemma_hash_verifiable_implies_induction_props_or_hash_collision_aux ils (I.length ils)
-  
+
 let lemma_time_seq_rw_consistent #vcfg
                                  (ils: IntTS.hash_verifiable_log vcfg {~ (rw_consistent (IntTS.to_state_ops ils))})
-  : hash_collision_gen = 
+  : hash_collision_gen =
   let ts_ops = IntTS.to_state_ops ils in
   let hc_or_props = lemma_hash_verifiable_implies_induction_props_or_hash_collision ils in
-  
+
   (* if hc_or_inv returns a hash collision, then we can return the same collision *)
   if Some? hc_or_props
     then Some?.v hc_or_props
 
   (* otherwise, we can use the spec-level lemma *)
-  else 
+  else
     let ilk = IntTS.to_logk ils in
     SpecC.lemma_time_seq_rw_consistent ilk
-  
+
 // final correctness property
 let lemma_verifier_correct (#vcfg:_) (gl: IntG.hash_verifiable_log vcfg { ~ (seq_consistent (IntG.to_state_ops gl))})
-  : hash_collision_gen = 
+  : hash_collision_gen =
   (* sequences of per-thread put/get operations *)
   let g_ops = IntG.to_state_ops gl in
-  
+
   (* sequence ordered by time of each log entry *)
-  let il = IntTS.create gl in  
+  let il = IntTS.create gl in
   I.lemma_interleaving_correct il;
   assert(I.interleave (I.i_seq il) gl);
 
